Rewrite a bit monoid.ec and add some distr lemma

theories/Monoid.ec
@@ -1,115 +1,147 @@
-type t.
+theory Comoid.
 
-op (+) : t -> t -> t.
+theory Base.
+  type t.
 
-op Z : t.
+  op (+) : t -> t -> t.
 
-axiom C : forall x y, x + y = y + x.
+  op Z : t.
 
-axiom A : forall x y z, x + (y + z) = x + y + z.
+  axiom C : forall x y, x + y = y + x.
 
-axiom addZ : forall x, x + Z = x.
+  axiom A : forall x y z, x + (y + z) = x + y + z.
 
-theory SumSet.
+  axiom addZ : forall x, x + Z = x.
+end Base.
+export Base.
 
-  require import FSet.
+require import FSet.
 
-  op sum(f:'a -> t, s:'a set) : t =
-    fold (lambda x s, s + (f x)) Z s.
+op sum(f:'a -> t, s:'a set) : t =
+  fold (lambda x s, s + (f x)) Z s.
 
-  lemma sum_nil:
-    forall (f:'a -> t), sum f empty = Z
-  by (intros=> ?;delta sum;simplify;apply fold_empty).
+lemma sum_empty: forall (f:'a -> t), sum f empty = Z
+by (intros=> ?;delta sum;simplify;apply fold_empty).
 
-  lemma sum_rm :
-    forall (f:'a -> t) (s:'a set) (x:'a),
+lemma sum_rm :
+  forall (f:'a -> t) (s:'a set) (x:'a),
     mem x s =>
     sum f s = (f x) + (sum f (rm x s)).
-  proof strict.
-    simplify sum.
-    intros ? ? ? ?.
-    rewrite (foldC x (lambda x s, s + (f x))) // /=.
-      by intros=> a b X;rewrite -A (C (f b)) A //.
-      by rewrite C //.
-  qed.
+proof strict.
+  simplify sum.
+  intros ? ? ? ?.
+  rewrite (foldC x (lambda x s, s + (f x))) // /=.
+    by intros=> a b X;rewrite -A (C (f b)) A //.
+    by rewrite C //.
+qed.
 
-  lemma sum_add :
-    forall (f:'a -> t) (s:'a set) (x:'a),
-    (!mem x s) =>
-    sum f (add x s) = (f x) + (sum f s).
-  proof strict.
-    intros ? ? ? ?.
-    rewrite (sum_rm _ _ x);first rewrite mem_add //.
-    by rewrite rm_add_eq -rm_nin_id //.
-  save.
+lemma sum_add :
+  forall (f:'a -> t) (s:'a set) (x:'a),
+  (!mem x s) =>
+  sum f (add x s) = (f x) + (sum f s).
+proof strict.
+  intros ? ? ? ?.
+  rewrite (sum_rm _ _ x);first rewrite mem_add //.
+  by rewrite rm_add_eq -rm_nin_id //.
+save.
 
-
-  lemma sum_in :
-    forall (f:'a -> t) (s:'a set),
+lemma sum_in :
+  forall (f:'a -> t) (s:'a set),
     sum f s = sum (lambda x, if mem x s then f x else Z) s.
-  proof.
-    intros ? ?.
-    pose {1 3} xs := s.
-    cut : (xs <= s);first by delta xs;apply leq_refl.
-    elim/set_comp xs;first rewrite ! sum_nil //.
-    intros ? ? ? ?.
-    rewrite (sum_rm _ _ (pick s0));
-      first by apply mem_pick.
-    rewrite (sum_rm<:'a> (lambda x, if mem x s then f x else Z) _ (pick s0));
-      first by apply mem_pick.
-    rewrite H0 /=;first by apply (leq_tran _ s0);
-      first apply rm_leq.
-    rewrite (_: mem (pick s0) s = true) //.
-    by apply eqT;apply H1;apply mem_pick=> //.
-  save.
+proof.
+  intros ? ?.
+  cut := leq_refl s.
+  pose {1 3 5} xs := s.
+  elim/set_comp xs;first by rewrite ! sum_empty //.
+  intros ? ? ? ?.
+  rewrite (sum_rm _ _ (pick s0));
+    first by apply mem_pick.
+  rewrite (sum_rm<:'a> (lambda x, if mem x s then f x else Z) _ (pick s0));
+    first by apply mem_pick.
+  rewrite H0 /=;first by apply (leq_tran _ s0);
+    first apply rm_leq.
+  rewrite (_: mem (pick s0) s = true) //.
+  by apply eqT;apply H1;apply mem_pick=> //.
+save.
 
-  lemma sum_add2 :
-    forall (f:'a -> t) (g:'a -> t) (s:'a set),
-    (sum f s) + (sum g s) = sum (lambda x, f x + g x) s.
-  proof.
-    intros ? ? ?.
-    elim/set_comp s;first rewrite ! sum_nil addZ //.
-    intros ? ? ?.
-    rewrite (sum_rm f _ (pick s0));first apply mem_pick;trivial.
-    rewrite (sum_rm g _ (pick s0));first apply mem_pick;trivial.
-    rewrite (sum_rm (lambda (x : 'a), f x + g x) _ (pick s0));first apply mem_pick;trivial.
-    rewrite -H0.
-    simplify.
-    by rewrite -A (A (sum f (rm (pick s0) s0))) (C (sum f (rm (pick s0) s0))) - !A !A //.
-  save.
+lemma sum_add2 :
+  forall (f:'a -> t) (g:'a -> t) (s:'a set),
+  (sum f s) + (sum g s) = sum (lambda x, f x + g x) s.
+proof.
+  intros ? ? ?.
+  elim/set_comp s;first by rewrite ! sum_empty addZ //.
+  intros ? ? ?.
+  rewrite (sum_rm f _ (pick s0));first apply mem_pick;trivial.
+  rewrite (sum_rm g _ (pick s0));first apply mem_pick;trivial.
+  rewrite (sum_rm (lambda (x : 'a), f x + g x) _ (pick s0));
+    first apply mem_pick=> //.
+  rewrite -H0 /=.
+  by rewrite -A (A (sum f (rm (pick s0) s0))) (C (sum f (rm (pick s0) s0))) - !A !A //.
+save.
 
-  lemma sum_chind :
-    forall (f:'a -> t) (g:'a -> 'a) (gg:'a -> 'a) (s:'a set),
-      (forall x, mem x s => gg (g x) = x) =>
-    (sum f s) = sum (lambda x, f (gg x)) (img g s).
-  proof.
-    intros ? ? ? ? ?.
-    pose xs := s.
-    cut lem : (xs <= s => (sum f xs) = sum (lambda x, f (gg x)) (img g xs));
-      last apply lem;delta xs;apply leq_refl.
-    elim/set_comp xs;first rewrite ! sum_nil //;
-      first rewrite img_empty;rewrite sum_nil;trivial.
-    intros ? ? ? ?.
-    rewrite (sum_rm _ _ (pick s0));first apply mem_pick;trivial.
-    rewrite (sum_rm _ (img g s0) (g (pick s0)));first apply mem_img;apply mem_pick;trivial.
-    simplify.
-    rewrite H;first apply H2;apply mem_pick;trivial.
-    rewrite H1;first apply (leq_tran _ s0);[apply rm_leq|trivial].
-    rewrite img_rm.
-    cut -> : (forall (x' : 'a), mem x' s0 => g (pick s0) = g x' => pick s0 = x') = true;last by trivial.
-    apply eqT=> x ? ?.
-    rewrite -H;first apply H2;apply mem_pick;trivial.
-    rewrite H4.
-    by apply H;first apply H2;trivial.
-  save.
-end SumSet.
+lemma sum_chind :
+  forall (f:'a -> t) (g:'a -> 'b) (gg:'b -> 'a) (s:'a set),
+    (forall x, mem x s => gg (g x) = x) =>
+  (sum f s) = sum (lambda x, f (gg x)) (img g s).
+proof.
+  intros ? ? ? ? ?.
+  cut := leq_refl s.
+  pose {1 3 4} xs := s.
+  elim/set_comp xs;first by rewrite ! sum_empty //;
+    first by rewrite img_empty;rewrite sum_empty //.
+  intros ? ? ? ?.
+  rewrite (sum_rm _ _ (pick s0));first apply mem_pick=> //.
+  rewrite (sum_rm _ (img g s0) (g (pick s0)));
+    first apply mem_img;apply mem_pick=> //.
+  simplify.
+  rewrite H;first apply H2;apply mem_pick;trivial.
+  rewrite H1;first apply (leq_tran _ s0);[apply rm_leq|trivial].
+  rewrite img_rm.
+  cut -> : (forall (x' : 'a), mem x' s0 => g (pick s0) = g x' => pick s0 = x') = true;last by trivial.
+  apply eqT=> x ? ?.
+  rewrite -H;first apply H2;apply mem_pick=> //.
+  rewrite H4.
+  by apply H;first apply H2=> //.
+save.
+
+lemma filter_empty : forall (p:'a -> bool), filter p empty = empty.
+proof strict.
+intros _.
+apply set_ext=> x.
+cut := mem_empty x.
+rewrite mem_filter -rw_neqF=> -> //.
+qed.
+
+lemma rm_filter : forall x (p:'a -> bool) s, rm x (filter p s) = filter p (rm x s).
+proof strict.
+intros x p s.
+apply set_ext=> a.
+rewrite mem_filter mem_rm mem_filter mem_rm.
+trivial.
+qed.
+
+lemma sum_filter :
+  forall (f:'a -> t) (p:'a -> bool) (s:'a set),
+    (forall x, (!p x) => f x = Z) =>
+  sum f (filter p s) = sum f s.
+proof strict.
+  intros f p s h.
+  cut := leq_refl s.
+  pose {1 3 4} xs := s.
+  elim/set_comp xs;first by rewrite filter_empty //.
+  intros s0 nempty sub hrec.
+  rewrite (sum_rm _ s0 (pick s0));
+    first by apply mem_pick=> //.
+  rewrite -sub;first apply (leq_tran _ s0);[apply rm_leq|trivial].
+  case (p (pick s0))=> ppick.
+    by rewrite (sum_rm _ (filter p s0) (pick s0)) ? rm_filter //;
+      first by rewrite mem_filter;split=> //;apply mem_pick=> //.
+    by rewrite h // -rm_filter C addZ -rm_nin_id // mem_filter -rw_nand ppick //.
+save.
 
 theory NatMul.
-  require import FSet.
   require import Int.
-  
-  import SumSet.
-  
+
   op ( * ) : int -> t -> t.
 
   axiom MulZ : forall (x:t), 0*x = Z.
@@ -123,7 +155,7 @@ theory NatMul.
     intros ? ? ? ?.
     pose xs := s.
     cut lem : xs <= s => sum f xs = (card xs)*k;last apply lem;delta xs;apply leq_refl.
-    elim/set_comp xs;first rewrite sum_nil card_empty=> ?;
+    elim/set_comp xs;first by rewrite sum_empty card_empty=> ?;
       first rewrite MulZ //.
     intros ? ? ? ?.
     rewrite (sum_rm _ _ (pick s0));first apply mem_pick;by trivial.
@@ -133,3 +165,192 @@ theory NatMul.
     rewrite -MulI //; smt.
   save.
 end NatMul.
+
+end Comoid.
+
+require Bool.
+clone Comoid.Base as Bbor with
+   type t = bool,
+   op (+) = (\/),
+   op Z = false
+   proof * by smt.
+
+require Real.
+clone Comoid.Base as Brplus with
+   type t = real,
+   op (+) = Real.(+),
+   op Z = 0%r
+   proof * by smt.
+
+clone Comoid as Mbor with theory Base = Bbor.
+clone Comoid as Mrplus with
+  theory Base = Brplus,
+  op NatMul.( * ) = lambda n, (Real.( * ) (n%r))
+  proof NatMul.* by smt.
+
+require import FSet.
+require import Distr.
+
+pred cpOrs (X:('a->bool) set) (x:'a) = Mbor.sum (lambda (P:'a->bool), P x) X.
+
+pred disj_or (X:('a->bool) set) =
+  forall x1 x2,  x1 <> x2 => mem x1 X => mem x2 X =>
+      forall a, x1 a => !(x2 a).
+
+lemma or_exists : forall (f:'a->bool) s,
+  (Mbor.sum f s) <=> (exists x, (mem x s /\ f x)).
+intros d s.
+apply iffI;
+  last by intros=> [x [h1 h2]];rewrite (Mbor.sum_rm _ _ x) // h2 /Mbor.Base.(+) /Bbor.(+) //.
+intros=> h.
+pose p := lambda x, mem x s /\ d x.
+change (exists x, p x).
+apply ex_for.
+delta p=> {p}.
+generalize h.
+apply absurd=> /= h.
+cut := FSet.leq_refl s.
+pose {1 3} xs := s.
+elim/set_ind xs;
+  first by rewrite Mbor.sum_empty //.
+intros x s' nmem hrec hleq.
+cut := h x.
+cut leq : (s' <= s) by (apply (FSet.leq_tran _ (add x s'))=> //;apply leq_add).
+rewrite Mbor.sum_add // /Mbor.Base.(+) /Bbor.(+) -rw_nor hrec // -rw_nand /=.
+case (mem x s)=> // /=.
+cut := hleq x.
+rewrite mem_add /= => -> //.
+qed.
+
+lemma mu_ors :
+  forall d (X:('a->bool) set), disj_or X =>
+    mu d (cpOrs X) = Mrplus.sum (lambda P, mu d P) X.
+proof strict.
+intros d X.
+elim/set_ind X => {X};
+  first by intros Hd;
+           rewrite Mrplus.sum_empty /Mrplus.Base.Z /Brplus.Z -(mu_false d);
+           apply mu_eq; rewrite /cpOrs=> x /=;
+           rewrite Mbor.sum_empty //.
+intros x X Hn Hr Hd.
+rewrite Mrplus.sum_add // /cpOrs.
+cut -> :
+  mu d  (lambda (x0 : 'a),
+    (Mbor.sum (lambda (P : 'a -> bool), P x0) (add x X))) =
+  mu d (cpOr x
+    (lambda x0, (Mbor.sum (lambda (P : 'a -> bool), P x0) X)))
+by (apply mu_eq => x0 /=;rewrite Mbor.sum_add //).
+rewrite mu_disjoint;
+  last by rewrite -Hr //;
+          intros p1 p2 H_1 H2 H3 b;
+          apply (Hd p1 p2 _ _ _ b)=> //;rewrite mem_add //;left;assumption.
+rewrite /cpAnd /cpFalse => x0 /=.
+rewrite -not_def => [H1 H2].
+generalize Hn Hd H2.
+elim/ set_ind X;first by rewrite Mbor.sum_empty /Mbor.Base.Z /Bbor.Z /=.
+intros x1 X' Hn' Hr' Hn Hd H2.
+cut H1' := Hd x x1 _ _ _ x0.
+  by rewrite -not_def=> Ht;generalize Ht Hn => ->;rewrite mem_add.
+  by rewrite mem_add.
+  by rewrite ! mem_add.
+generalize H2; rewrite Mbor.sum_add //=.
+cut Hd': disj_or (add x X') by (
+  rewrite /disj_or;
+  intros a1 a2;
+  rewrite ! mem_add;
+  intros Hneq Hm1 Hm2;
+  apply Hd;[
+    assumption |
+    rewrite ! mem_add -/Bbor.(+) -Bbor.A (Bbor.C (a1 = x1)) Bbor.A /Bbor.(+);left;assumption |
+    rewrite ! mem_add -/Bbor.(+) -Bbor.A (Bbor.C (a2 = x1)) Bbor.A /Bbor.(+);left;assumption]).
+rewrite /Mbor.Base.(+) /Bbor.(+) -(nnot (x1 x0)) H1' ?H1 // /= -not_def.
+apply Hr'=> //.
+generalize Hn.
+rewrite mem_add -rw_nor //.
+save.
+
+require ISet.
+import Real.
+lemma mean :
+  forall (d:'a distr) (p:'a -> bool),
+    ISet.Finite.finite (ISet.support d) =>
+    d <> Dempty.dempty =>
+    mu d p = Mrplus.sum (lambda x, (mu_x d x)*(mu (Dunit.dunit x) p)) (ISet.Finite.toFSet (ISet.support d)).
+proof strict.
+intros=> d p finite nEmpty.
+pose s := FSet.filter p (ISet.Finite.toFSet (ISet.support d)).
+pose pi := lambda (a:'a) (b:'a), a = b.
+pose piI := lambda (x:'a -> bool), pick (FSet.filter x s).
+pose is := img pi s.
+cut bij1 : forall x, mem x s => piI (pi x) = x.
+  delta piI pi.
+  intros x h /=.
+  apply (_:forall a, mem a (filter (lambda (b : 'a), x = b) s) => a = x);
+    first by (intros=> a;rewrite mem_filter //).
+  rewrite mem_pick //.
+  smt.
+cut bij2 : forall x, mem x is => pi (piI x) = x.
+  delta piI pi.
+  intros x h /=.
+  apply fun_ext=> a /=.
+  smt.
+cut p_is_or : mu d p = mu d (cpOrs is).
+  rewrite /cpOrs /is mu_in_supp /cpAnd /=.
+  congr=> //.
+  apply fun_ext=> x /=.
+  rewrite or_exists andC.
+  case (in_supp x d /\ p x)=>h.
+    rewrite rw_eq_sym rw_eqT.
+    exists (pi x).
+    split;last by delta pi=> //.
+    by rewrite /s mem_img // mem_filter ISet.Finite.mem_toFSet // /ISet.support ISet.mem_create //.
+
+    rewrite rw_eq_sym rw_neqF.
+    pose q := (lambda x0, mem x0 (img pi s) /\ x0 x).
+    change (! exists x, q x).
+    apply nexists.
+    intros a.
+    delta q=> /= {q}.
+    rewrite -rw_nand -/is.
+    case (mem a is)=> // /= hmem.
+    cut valA :pi (piI a) = a by (apply bij2=> //).
+    generalize hmem.
+    rewrite /is /s img_def.
+    intros [y [<-]].
+    rewrite mem_filter ISet.Finite.mem_toFSet // /ISet.support ISet.mem_create /=.
+    delta pi=> /=.
+    by apply absurd=> /= -> //.
+cut disj_or_is : disj_or is.
+  rewrite /disj_or /is.
+  intros x1 x2 h.
+  rewrite ! img_def=> [a1 [rh1 h1]] [a2 [rh2 h2]].
+  intros x.
+  generalize h.
+  rewrite -rh1 -rh2.
+  delta pi=> /=.
+  rewrite (rw_imp (a1=x)) rw_nand.
+  apply absurd=> /= h.
+  apply fun_ext=> y /=.
+by generalize h=> [-> ->] //.
+
+rewrite p_is_or mu_ors //.
+rewrite -(Mrplus.sum_filter _ p);
+  first by intros x h /=;rewrite Dunit.mu_def_notin //.
+rewrite -/s (Mrplus.sum_chind _ pi piI) // /= -/is Mrplus.sum_in rw_eq_sym Mrplus.sum_in rw_eq_sym.
+congr=> //;apply fun_ext=> P /=.
+rewrite /mu_x.
+case (mem P is)=> memP //.
+case (p (piI P))=> h.
+  rewrite Dunit.mu_def_in // -{1}(bij2 P) //.
+  delta pi=> /=.
+  congr=> //.
+  by apply fun_ext=> //.
+
+  rewrite Dunit.mu_def_notin //.
+  cut : (P = cpFalse);last smt.
+  apply fun_ext.
+  intros=> x.
+  rewrite -(bij2 P) //.
+  simplify pi.
+  smt.
+save.
